Removing parts of the compiler

driver/Compiler.v
@@ -161,6 +161,13 @@ Definition transf_clight_program (p: Clight.program) : res Asm.program :=
   @@@ time "Cminor generation" Cminorgen.transl_program
   @@@ transf_cminor_program.
 
+Definition simpl_transf_clight_program (p: Clight.program) : res Asm.program :=
+  OK p
+   @@ print print_Clight
+  @@@ time "C#minor generation" Cshmgen.transl_program
+  @@@ time "Cminor generation" Cminorgen.transl_program
+  @@@ transf_cminor_program.
+
 Definition transf_c_program (p: Csyntax.program) : res Asm.program :=
   OK p
   @@@ time "Clight generation" SimplExpr.transl_program
@@ -252,6 +259,29 @@ Definition CompCert's_passes :=
   ::: mkpass Asmgenproof.match_prog
   ::: pass_nil _.
 
+
+Definition Simpl_CompCert's_passes :=
+      mkpass Cshmgenproof.match_prog
+  ::: mkpass Cminorgenproof.match_prog
+  ::: mkpass Selectionproof.match_prog
+  ::: mkpass RTLgenproof.match_prog
+  ::: mkpass (match_if Compopts.optim_tailcalls Tailcallproof.match_prog)
+  ::: mkpass Inliningproof.match_prog
+  ::: mkpass Renumberproof.match_prog
+  ::: mkpass (match_if Compopts.optim_constprop Constpropproof.match_prog)
+  ::: mkpass (match_if Compopts.optim_constprop Renumberproof.match_prog)
+  ::: mkpass (match_if Compopts.optim_CSE CSEproof.match_prog)
+  ::: mkpass (match_if Compopts.optim_redundancy Deadcodeproof.match_prog)
+  ::: mkpass Unusedglobproof.match_prog
+  ::: mkpass Allocproof.match_prog
+  ::: mkpass Tunnelingproof.match_prog
+  ::: mkpass Linearizeproof.match_prog
+  ::: mkpass CleanupLabelsproof.match_prog
+  ::: mkpass (match_if Compopts.debug Debugvarproof.match_prog)
+  ::: mkpass Stackingproof.match_prog
+  ::: mkpass Asmgenproof.match_prog
+  ::: pass_nil _.
+
 (** Composing the [match_prog] relations above, we obtain the relation
   between CompCert C sources and Asm code that characterize CompCert's
   compilation. *)
@@ -259,8 +289,64 @@ Definition CompCert's_passes :=
 Definition match_prog: Csyntax.program -> Asm.program -> Prop :=
   pass_match (compose_passes CompCert's_passes).
 
+Definition simpl_match_prog: Clight.program -> Asm.program -> Prop :=
+  pass_match (compose_passes Simpl_CompCert's_passes).
+
 (** The [transf_c_program] function, when successful, produces
   assembly code that is in the [match_prog] relation with the source C program. *)
+
+Theorem transf_clight_program_match:
+  forall p tp,
+  simpl_transf_clight_program p = OK tp ->
+  simpl_match_prog p tp.
+Proof.
+  intros p tp T.
+  unfold simpl_transf_clight_program, time in T.
+  rewrite ! compose_print_identity in T. simpl in T.
+  destruct (Cshmgen.transl_program p) as [p3|e] eqn:P3; simpl in T; try discriminate.
+  destruct (Cminorgen.transl_program p3) as [p4|e] eqn:P4; simpl in T; try discriminate.
+  unfold transf_cminor_program, time in T. rewrite ! compose_print_identity in T. simpl in T.
+  destruct (Selection.sel_program p4) as [p5|e] eqn:P5; simpl in T; try discriminate.
+  destruct (RTLgen.transl_program p5) as [p6|e] eqn:P6; simpl in T; try discriminate.
+  unfold transf_rtl_program, time in T. rewrite ! compose_print_identity in T. simpl in T.
+  set (p7 := total_if optim_tailcalls Tailcall.transf_program p6) in *.
+  destruct (Inlining.transf_program p7) as [p8|e] eqn:P8; simpl in T; try discriminate.
+  set (p9 := Renumber.transf_program p8) in *.
+  set (p10 := total_if optim_constprop Constprop.transf_program p9) in *.
+  set (p11 := total_if optim_constprop Renumber.transf_program p10) in *.
+  destruct (partial_if optim_CSE CSE.transf_program p11) as [p12|e] eqn:P12; simpl in T; try discriminate.
+  destruct (partial_if optim_redundancy Deadcode.transf_program p12) as [p13|e] eqn:P13; simpl in T; try discriminate.
+  destruct (Unusedglob.transform_program p13) as [p14|e] eqn:P14; simpl in T; try discriminate.
+  destruct (Allocation.transf_program p14) as [p15|e] eqn:P15; simpl in T; try discriminate.
+  set (p16 := Tunneling.tunnel_program p15) in *.
+  destruct (Linearize.transf_program p16) as [p17|e] eqn:P17; simpl in T; try discriminate.
+  set (p18 := CleanupLabels.transf_program p17) in *.
+  destruct (partial_if debug Debugvar.transf_program p18) as [p19|e] eqn:P19; simpl in T; try discriminate.
+  destruct (Stacking.transf_program p19) as [p20|e] eqn:P20; simpl in T; try discriminate.
+  unfold match_prog; simpl. 
+  exists p3; split. apply Cshmgenproof.transf_program_match; auto.
+  exists p4; split. apply Cminorgenproof.transf_program_match; auto.
+  exists p5; split. apply Selectionproof.transf_program_match; auto.
+  exists p6; split. apply RTLgenproof.transf_program_match; auto.
+  exists p7; split. apply total_if_match. apply Tailcallproof.transf_program_match.
+  exists p8; split. apply Inliningproof.transf_program_match; auto.
+  exists p9; split. apply Renumberproof.transf_program_match; auto.
+  exists p10; split. apply total_if_match. apply Constpropproof.transf_program_match.
+  exists p11; split. apply total_if_match. apply Renumberproof.transf_program_match.
+  exists p12; split. eapply partial_if_match; eauto. apply CSEproof.transf_program_match.
+  exists p13; split. eapply partial_if_match; eauto. apply Deadcodeproof.transf_program_match.
+  exists p14; split. apply Unusedglobproof.transf_program_match; auto.
+  exists p15; split. apply Allocproof.transf_program_match; auto.
+  exists p16; split. apply Tunnelingproof.transf_program_match.
+  exists p17; split. apply Linearizeproof.transf_program_match; auto.
+  exists p18; split. apply CleanupLabelsproof.transf_program_match; auto.
+  exists p19; split. eapply partial_if_match; eauto. apply Debugvarproof.transf_program_match.
+  exists p20; split. apply Stackingproof.transf_program_match; auto.
+  exists tp; split. apply Asmgenproof.transf_program_match; auto. 
+  reflexivity.
+Qed.
+
+
 
 Theorem transf_c_program_match:
   forall p tp,
@@ -349,6 +435,65 @@ Lemma match_if_simulation:
 Proof.
   intros. unfold match_if in *. destruct (flag tt). eauto. subst. apply forward_simulation_identity.
 Qed.
+
+
+Theorem simpl_clight_semantic_preservation:
+  forall p tp,
+  simpl_match_prog p tp ->
+  forward_simulation (Clight.semantics2 p) (Asm.semantics tp).
+Proof.
+  intros p tp M. unfold simpl_match_prog, pass_match in M; simpl in M.
+Ltac DestructM' :=
+  match goal with
+    [ H: exists p, _ /\ _ |- _ ] => 
+      let p := fresh "p" in let M := fresh "M" in let MM := fresh "MM" in
+      destruct H as (p & M & MM); clear H
+  end.
+  repeat DestructM'. subst tp.
+  assert (F: forward_simulation (Clight.semantics2 p) (Asm.semantics p19)).
+  {
+   eapply compose_forward_simulations.
+    eapply Cshmgenproof.transl_program_correct; eassumption.
+  eapply compose_forward_simulations.
+    eapply Cminorgenproof.transl_program_correct; eassumption.
+  eapply compose_forward_simulations.
+    eapply Selectionproof.transf_program_correct; eassumption.
+  eapply compose_forward_simulations.
+    eapply RTLgenproof.transf_program_correct; eassumption.
+  eapply compose_forward_simulations.
+    eapply match_if_simulation. eassumption. exact Tailcallproof.transf_program_correct.
+  eapply compose_forward_simulations.
+    eapply Inliningproof.transf_program_correct; eassumption.
+  eapply compose_forward_simulations. eapply Renumberproof.transf_program_correct; eassumption.
+  eapply compose_forward_simulations.
+    eapply match_if_simulation. eassumption. exact Constpropproof.transf_program_correct.
+  eapply compose_forward_simulations.
+    eapply match_if_simulation. eassumption. exact Renumberproof.transf_program_correct.
+  eapply compose_forward_simulations.
+    eapply match_if_simulation. eassumption. exact CSEproof.transf_program_correct.
+  eapply compose_forward_simulations.
+    eapply match_if_simulation. eassumption. exact Deadcodeproof.transf_program_correct; eassumption.
+  eapply compose_forward_simulations.
+    eapply Unusedglobproof.transf_program_correct; eassumption.
+  eapply compose_forward_simulations.
+    eapply Allocproof.transf_program_correct; eassumption.
+  eapply compose_forward_simulations.
+    eapply Tunnelingproof.transf_program_correct; eassumption.
+  eapply compose_forward_simulations.
+    eapply Linearizeproof.transf_program_correct; eassumption.
+  eapply compose_forward_simulations.
+    eapply CleanupLabelsproof.transf_program_correct; eassumption.
+  eapply compose_forward_simulations.
+    eapply match_if_simulation. eassumption. exact Debugvarproof.transf_program_correct.
+  eapply compose_forward_simulations.
+    eapply Stackingproof.transf_program_correct with (return_address_offset := Asmgenproof0.return_address_offset).
+    exact Asmgenproof.return_address_exists.
+    eassumption.
+  eapply Asmgenproof.transf_program_correct; eassumption.
+  }
+  auto.
+Qed.
+
 
 Theorem cstrategy_semantic_preservation:
   forall p tp,
